Validator/Regex/Lang.lean
@@ -2,6 +2,9 @@ import Validator.Std.List
 
 def Lang (α: Type): Type := List α → Prop
 
+def Lang.MemFilter {α: Type} (R: Lang α) (xss: List (List α)): Lang α :=
+  fun xs => xs ∈ xss /\ R xs
+
 def Lang.emptyset: Lang α := fun _ => False
 def Lang.emptystr: Lang α := fun xs => xs = []
 def Lang.symbol (Φ: σ → α → Prop) (s: σ): Lang α :=
